completeness

VeryWeakSubintuitionistic/FMT/Basic.lean
@@ -4,39 +4,41 @@ public import VeryWeakSubintuitionistic.Proof.VF
 
 @[expose] public section
 
-structure FMTFrame (κ : Type*) (α : Type*) where
+namespace FMTSemantics
+
+structure Frame (κ : Type*) (α : Type*) where
   Rel' : Formula α → κ → κ → Prop
   root' : κ
   root_rooted' : ∀ {A x}, Rel' A root' x
 
-namespace FMTFrame
+namespace Frame
 
-variable {κ α : Type*} {F : FMTFrame κ α}
+variable {κ α : Type*} {F : Frame κ α}
 
-abbrev World (_ : FMTFrame κ α) := κ
-abbrev Rel {F : FMTFrame κ α} (A : Formula α) (x y : F.World) := F.Rel' A x y
-notation:45 x:90 " ≺[" φ "] " y:90 => FMTFrame.Rel φ x y
+abbrev World (_ : Frame κ α) := κ
+abbrev Rel {F : Frame κ α} (A : Formula α) (x y : F.World) := F.Rel' A x y
+notation:45 x:90 " ≺[" φ "] " y:90 => Frame.Rel φ x y
 
 abbrev root : F.World := F.root'
 @[grind .] lemma root_rooted : ∀ {A x}, F.root ≺[A] x := F.root_rooted'
 
-end FMTFrame
+end Frame
 
 
-structure FMTModel (κ : Type*) (α : Type*) extends FMTFrame κ α where
-  Val : α → (toFMTFrame.World) → Prop
+structure Model (κ : Type*) (α : Type*) extends Frame κ α where
+  Val : α → (toFrame.World) → Prop
 
-namespace FMTModel
+namespace Model
 
-instance : CoeFun (FMTModel κ α) (λ M => α → M.World → Prop) := ⟨fun m => m.Val⟩
+instance : CoeFun (Model κ α) (λ M => α → M.World → Prop) := ⟨fun m => m.Val⟩
 
-end FMTModel
+end Model
 
 
-variable {κ α : Type*} {M : FMTModel κ α} {A B C : Formula α}
+variable {κ α : Type*} {M : Model κ α} {A B C : Formula α}
 
 @[grind]
-def Forces {M : FMTModel κ α} (x : M.World) : Formula α → Prop
+def Forces {M : Model κ α} (x : M.World) : Formula α → Prop
   | #a     => M a x
   | ⊥      => False
   | A ⋏ B   => Forces x A ∧ Forces x B
@@ -44,102 +46,129 @@ def Forces {M : FMTModel κ α} (x : M.World) : Formula α → Prop
   | A 🡒 B => ∀ y, x ≺[A 🡒 B] y → (Forces y A → Forces y B)
 infix:45 " ⊩ " => Forces
 
-abbrev NotForces {M : FMTModel κ α} (x : M.World) (φ : Formula α) : Prop := ¬(x ⊩ φ)
+abbrev NotForces {M : Model κ α} (x : M.World) (φ : Formula α) : Prop := ¬(x ⊩ φ)
 infix:45 " ⊮ " => NotForces
 
 lemma iff_not_Forces_imp : (x ⊮ A 🡒 B) ↔ (∃ y, x ≺[A 🡒 B] y ∧ (y ⊩ A ∧ y ⊮ B)) := by
   simp [NotForces, Forces];
 
+@[simp, grind .] lemma forces_top : x ⊩ ⊤ := by intro y; simp;
 
-@[grind] def Validates (M : FMTModel κ α) (A : Formula α) : Prop := ∀ x : M.World, x ⊩ A
+
+@[grind] def Validates (M : Model κ α) (A : Formula α) : Prop := ∀ x : M.World, x ⊩ A
 infix:45 " ⊨ " => Validates
 
-@[grind] abbrev NotValidates (M : FMTModel κ α) (A : Formula α) : Prop := ¬(M ⊨ A)
+@[grind] abbrev NotValidates (M : Model κ α) (A : Formula α) : Prop := ¬(M ⊨ A)
 infix:45 " ⊭ " => NotValidates
 
-lemma iff_Valid_exists_world_not_Forces {M : FMTModel κ α} {A : Formula α} : (M ⊭ A) ↔ (∃ x : M.World, x ⊮ A) := by
+lemma iff_Valid_exists_world_not_Forces {M : Model κ α} {A : Formula α} : (M ⊭ A) ↔ (∃ x : M.World, x ⊮ A) := by
   simp only [NotValidates, Validates, not_forall, NotForces];
 
 
-@[grind] def FMTFrameValid (F : FMTFrame κ α) (A : Formula α) : Prop := ∀ V, Validates ⟨F, V⟩ A
-infix:45 " ⊨ " => FMTFrameValid
+@[grind] def FrameValid (F : Frame κ α) (A : Formula α) : Prop := ∀ V, Validates ⟨F, V⟩ A
+infix:45 " ⊨ " => FrameValid
 
-abbrev NotFMTFrameValid (F : FMTFrame κ α) (A : Formula α) : Prop := ¬(F ⊨ A)
-infix:45 " ⊭ " => NotFMTFrameValid
+abbrev NotFrameValid (F : Frame κ α) (A : Formula α) : Prop := ¬(F ⊨ A)
+infix:45 " ⊭ " => NotFrameValid
 
-lemma iff_notFMTFrameValid_exists_model_world {F : FMTFrame κ α} {A : Formula α} : (F ⊭ A) ↔ (∃ V, ∃ x : (⟨F, V⟩ : FMTModel κ α).World, x ⊮ A) := by
-  simp only [NotFMTFrameValid, FMTFrameValid, Validates, not_forall, NotForces];
+lemma iff_notFrameValid_exists_model_world {F : Frame κ α} {A : Formula α} : (F ⊭ A) ↔ (∃ V, ∃ x : (⟨F, V⟩ : Model κ α).World, x ⊮ A) := by
+  simp only [NotFrameValid, FrameValid, Validates, not_forall, NotForces];
 
 
 section Soundness
 
-variable {κ α : Type*} {M : FMTModel κ α} {A B C : Formula α}
+variable {κ α : Type*} {F : Frame κ α} {M : Model κ α} {A B C : Formula α}
 
-@[grind .] lemma valid_andElimL : M ⊨ (A ⋏ B) 🡒 A := by grind;
-@[grind .] lemma valid_andElimR : M ⊨ (A ⋏ B) 🡒 B := by grind;
-@[grind .] lemma valid_orIntroL : M ⊨ A 🡒 (A ⋎ B) := by grind;
-@[grind .] lemma valid_orIntroR : M ⊨ B 🡒 (A ⋎ B) := by grind;
-@[grind .] lemma valid_distributeAndOr : M ⊨ (A ⋏ (B ⋎ C)) 🡒 ((A ⋏ B) ⋎ (A ⋏ C)) := by grind;
-@[grind .] lemma valid_impId : M ⊨ A 🡒 A := by grind;
-@[grind .] lemma valid_efq : M ⊨ ⊥ 🡒 A := by grind;
+@[grind .] lemma frameValid_andElimL : F ⊨ (A ⋏ B) 🡒 A := by grind;
+@[grind .] lemma frameValid_andElimR : F ⊨ (A ⋏ B) 🡒 B := by grind;
+@[grind .] lemma frameValid_orIntroL : F ⊨ A 🡒 (A ⋎ B) := by grind;
+@[grind .] lemma frameValid_orIntroR : F ⊨ B 🡒 (A ⋎ B) := by grind;
+@[grind .] lemma frameValid_distributeAndOr : F ⊨ (A ⋏ (B ⋎ C)) 🡒 ((A ⋏ B) ⋎ (A ⋏ C)) := by grind;
+@[grind .] lemma frameValid_impId : F ⊨ A 🡒 A := by grind;
+@[grind .] lemma frameValid_efq : F ⊨ ⊥ 🡒 A := by grind;
+
+@[simp, grind .]
+lemma not_frameValid_bot : F ⊭ ⊥ := by
+  intro h;
+  have := @h (λ _ _ => True) F.root;
+  contradiction;
+
 
 @[grind <=]
-lemma valid_ruleI (hAB : M ⊨ A 🡒 B) (hBC : M ⊨ B 🡒 C) : M ⊨ A 🡒 C := by
+lemma frameValid_ruleI (hAB : F ⊨ A 🡒 B) (hBC : F ⊨ B 🡒 C) : F ⊨ A 🡒 C := by
+  intro V x y Rxy hya;
+  exact hBC V F.root y (by grind) $ hAB V F.root y (by grind) hya;
+
+@[grind <=]
+lemma frameValid_ruleC (hAB : F ⊨ A 🡒 B) (hAC : F ⊨ A 🡒 C) : F ⊨ A 🡒 (B ⋏ C) := by
+  intro V x y Rxy hya;
+  have := hAB V F.root y (by grind) hya;
+  have := hAC V F.root y (by grind) hya;
+  grind;
+
+@[grind <=]
+lemma frameValid_ruleD (hAC : F ⊨ A 🡒 C) (hBC : F ⊨ B 🡒 C) : F ⊨ (A ⋎ B) 🡒 C := by
+  rintro V x y Rxy (h | h);
+  . exact hAC V F.root y (by grind) h;
+  . exact hBC V F.root y (by grind) h;
+
+@[grind =>]
+lemma frameValid_mdp (hAB : F ⊨ A 🡒 B) (hA : F ⊨ A) : F ⊨ B := by
+  intro V x;
+  exact hAB V F.root x (show F.root ≺[A 🡒 B] x by grind) (by grind);
+
+@[grind <=]
+lemma frameValid_af (hA : F ⊨ A) : F ⊨ B 🡒 A := by grind;
+
+theorem soundness_frame : (Λ ⊢ⱽ A) → (∀ {κ}, ∀ F : Frame κ α, (∀ B ∈ Λ, F ⊨ B) → F ⊨ A) := by
+  intro h _ F hΛ; induction h <;> grind;
+
+
+
+@[grind <=]
+lemma modelValid_ruleI (hAB : M ⊨ A 🡒 B) (hBC : M ⊨ B 🡒 C) : M ⊨ A 🡒 C := by
   intro x y Rxy hya;
   exact hBC M.root y (by grind) $ hAB M.root y (by grind) hya;
 
 @[grind <=]
-lemma valid_ruleC (hAB : M ⊨ A 🡒 B) (hAC : M ⊨ A 🡒 C) : M ⊨ A 🡒 (B ⋏ C) := by
+lemma modelValid_ruleC (hAB : M ⊨ A 🡒 B) (hAC : M ⊨ A 🡒 C) : M ⊨ A 🡒 (B ⋏ C) := by
   intro x y Rxy hya;
   have := hAB M.root y (by grind) hya;
   have := hAC M.root y (by grind) hya;
   grind;
 
 @[grind <=]
-lemma valid_ruleD (hAC : M ⊨ A 🡒 C) (hBC : M ⊨ B 🡒 C) : M ⊨ (A ⋎ B) 🡒 C := by
+lemma modelValid_ruleD (hAC : M ⊨ A 🡒 C) (hBC : M ⊨ B 🡒 C) : M ⊨ (A ⋎ B) 🡒 C := by
   rintro x y Rxy (h | h);
   . exact hAC M.root y (by grind) h;
   . exact hBC M.root y (by grind) h;
 
 @[grind =>]
-lemma valid_mdp (hAB : M ⊨ A 🡒 B) (hA : M ⊨ A) : M ⊨ B := by
+lemma modelValid_mdp (hAB : M ⊨ A 🡒 B) (hA : M ⊨ A) : M ⊨ B := by
   intro x;
-  exact hAB _ x (show M.root ≺[A 🡒 B] x by grind) (by grind);
+  exact hAB M.root x (show M.root ≺[A 🡒 B] x by grind) (by grind);
 
 @[grind <=]
-lemma valid_af (hA : M ⊨ A) : M ⊨ B 🡒 A := by grind;
+lemma modelValid_af (hA : M ⊨ A) : M ⊨ B 🡒 A := by grind;
 
-theorem soundness : (Λ ⊢ⱽ A) → (∀ {κ}, ∀ M : FMTModel κ α, (∀ φ ∈ Λ, M ⊨ φ) → M ⊨ A) := by
-  intro h _ M hΛ; induction h <;> grind;
+theorem soundness_model : (Λ ⊢ⱽ A) → (∀ {κ}, ∀ M : Model κ α, (∀ B ∈ Λ, M ⊨ B) → M ⊨ A) := by
+  intro h _ M hM; induction h <;> grind;
 
 
-@[grind .]
+
+@[simp, grind .]
 theorem consistency_of_VF : (∅ ⊬ (⊥ : Formula α)) := by
   by_contra!;
-  let M : FMTModel (Fin 1) α := {
+  let F : Frame (Fin 1) α := {
     Rel' := λ _ _ _ => True,
     root' := 1,
     root_rooted' := by grind;
-    Val := λ _ _ => True
   };
-  have : (1 : M.World) ⊩ ⊥ := soundness this M (by grind) _;
-  contradiction;
-
-@[grind .]
-theorem consistency_VF : (∅ ⊬ (⊥ : Formula α)) := by
-  by_contra!;
-  let M : FMTModel (Fin 1) α := {
-    Rel' := λ _ _ _ => True,
-    root' := 1,
-    root_rooted' := by grind;
-    Val := λ _ _ => True
-  };
-  have : (1 : M.World) ⊩ ⊥ := soundness this M (by grind) _;
-  contradiction;
+  simpa using soundness_frame this F (by grind);
 
 example : (∅ ⊬ (⊤ 🡒 (#0 ⋏ #1) 🡘 (⊤ 🡒 (#1 ⋏ #0)))) := by
   by_contra!;
-  let M : FMTModel (Fin 3) ℕ := {
+  let M : Model (Fin 3) ℕ := {
     Rel' := λ A x y =>
       match A with
       | (⊤ 🡒 (#0 ⋏ #1)) => x ≠ 1
@@ -153,7 +182,7 @@ example : (∅ ⊬ (⊤ 🡒 (#0 ⋏ #1) 🡘 (⊤ 🡒 (#1 ⋏ #0)))) := by
       | 0 => x = 2
       | _ => False
   };
-  have : (0 : M.World) ⊩ (⊤ 🡒 (#0 ⋏ #1) 🡘 (⊤ 🡒 (#1 ⋏ #0))) := soundness this M (by grind) 0;
+  have : (0 : M.World) ⊩ (⊤ 🡒 (#0 ⋏ #1) 🡘 (⊤ 🡒 (#1 ⋏ #0))) := soundness_model this M (by grind) 0;
   have : (2 : M.World) ⊩ #1 := @this.1 1 (by grind) (by grind) 2 (by grind) (by grind) |>.1;
   contradiction;
 
@@ -163,36 +192,52 @@ end Soundness
 section
 
 @[grind]
-def FMTFrameForces {F : FMTFrame κ α} (x : F.World) (A : Formula α) (A_closed : A.Closed := by grind) : Prop :=
+def FrameForces {F : Frame κ α} (x : F.World) (A : Formula α) (A_closed : A.Closed := by grind) : Prop :=
   match A with
   | ⊥ => False
-  | A ⋏ B => FMTFrameForces x A ∧ FMTFrameForces x B
-  | A ⋎ B => FMTFrameForces x A ∨ FMTFrameForces x B
-  | A 🡒 B => ∀ {y}, F.Rel (A 🡒 B) x y → (FMTFrameForces y A → FMTFrameForces y B)
+  | A ⋏ B => FrameForces x A ∧ FrameForces x B
+  | A ⋎ B => FrameForces x A ∨ FrameForces x B
+  | A 🡒 B => ∀ {y}, F.Rel (A 🡒 B) x y → (FrameForces y A → FrameForces y B)
 
-variable {F : FMTFrame κ α}
+variable {F : Frame κ α}
+
+@[simp, grind .]
+lemma frameForces_top : FrameForces x (⊤ : Formula α) := by grind;
 
 @[grind =_]
-lemma iff_FMTFrameForces_Forces_of_closed {F : FMTFrame κ α} {x : F.World} {V} {A} (A_closed : A.Closed) : FMTFrameForces x A ↔ (Forces (M := ⟨F, V⟩) x A) := by
+lemma iff_FrameForces_Forces_of_closed {F : Frame κ α} {x : F.World} {V} {A} (A_closed : A.Closed) : FrameForces x A ↔ (Forces (M := ⟨F, V⟩) x A) := by
   induction A generalizing x <;> grind;
 
-lemma iff_Forces_CNA (A_closed : A.Closed) : FMTFrameValid F (∼A) ↔ ∀ x : F.World, ¬(FMTFrameForces x A) := by
+lemma iff_forces_of_closed {x : F.World} (A_closed : A.Closed) : (Forces (M := ⟨F, V⟩) x A) ↔ (Forces (M := ⟨F, V'⟩) x A) := by
+  simp [←iff_FrameForces_Forces_of_closed A_closed];
+
+lemma iff_FrameValid_ModelValid_of_closed {M : Model κ α} (A_closed : A.Closed) : (M.toFrame ⊨ A) ↔ (M ⊨ A) := by
+  constructor;
+  . intro h x;
+    apply h;
+  . intro h V x;
+    exact iff_forces_of_closed A_closed |>.mpr (@h x);
+
+lemma iff_FrameValid_neg_of_closed (A_closed : A.Closed) : F ⊨ (∼A) ↔ ∀ x : F.World, ¬(FrameForces x A) := by
   constructor;
   . intro h x;
     by_contra!
-    exact h (λ _ _ => True) F.root x (by grind) $ iff_FMTFrameForces_Forces_of_closed (by grind) |>.mp this;
+    exact h (λ _ _ => True) F.root x (by grind) $ iff_FrameForces_Forces_of_closed (by grind) |>.mp this;
   . intro h V x;
     grind;
 
 @[grind =_]
-lemma iff_closed_not_and : F ⊨ ∼(A ⋎ B) ↔ (FMTFrameValid F (∼A) ∧ FMTFrameValid F (∼B)) := by grind;
+lemma iff_frameValid_not_or : F ⊨ ∼(A ⋎ B) ↔ (F ⊨ ∼A ∧ F ⊨ ∼B) := by grind;
 
-lemma iff_closed_not_imp (A_closed : A.Closed) (B_closed : B.Closed) : F ⊨ ∼(A 🡒 B) ↔ (∀ x : F.World, ∃ y : F.World, x ≺[A 🡒 B] y ∧ (FMTFrameForces y A ∧ ¬FMTFrameForces y B)) := by
-  apply Iff.trans (iff_Forces_CNA (A := A 🡒 B) (by grind));
-  simp [FMTFrameForces];
+lemma iff_frameValid_closed_imp (A_closed : A.Closed) (B_closed : B.Closed)
+  : F ⊨ ∼(A 🡒 B) ↔ (∀ x : F.World, ∃ y : F.World, x ≺[A 🡒 B] y ∧ (FrameForces y A ∧ ¬FrameForces y B)) := by
+  apply Iff.trans (iff_FrameValid_neg_of_closed (A := A 🡒 B) (by grind));
+  simp [FrameForces];
 
-lemma iff_closed_dn (A_closed : A.Closed) : F ⊨ ∼∼A ↔ (∀ x : F.World, ∃ y : F.World, x ≺[∼A] y ∧ (FMTFrameForces y A)) := by
-  apply Iff.trans (iff_closed_not_imp (A := A) (B := ⊥) (by grind) (by grind));
-  simp [FMTFrameForces];
+lemma iff_frameValid_closed_dn (A_closed : A.Closed) : F ⊨ ∼∼A ↔ (∀ x : F.World, ∃ y : F.World, x ≺[∼A] y ∧ (FrameForces y A)) := by
+  apply Iff.trans (iff_frameValid_closed_imp (A := A) (B := ⊥) (by grind) (by grind));
+  simp [FrameForces];
 
 end
+
+end FMTSemantics
